refactor binencoders into multiple files

src/BinEncoders/Specs.v
@@ -1,50 +1,24 @@
-Require Import Coq.Strings.Ascii.
-Require Import Coq.Lists.List.
+Require Export Coq.Lists.List.
 
 Set Implicit Arguments.
 
-Definition bin := list bool.
+Section Specifications.
 
-Definition encode_decode_correct
-           (data_t : Type)
-           (encode : data_t -> bin)
-           (decode : bin -> data_t) :=
-  forall data, decode (encode data) = data.
+  Variable (data_t : Type)
+           (bin_t  : Type).
 
-Infix "<+>" := encode_decode_correct (at level 20, no associativity).
+  Definition encode_decode_correct
+             (predicate : data_t -> Prop)
+             (encode : data_t -> bin_t)
+             (decode : bin_t -> data_t) :=
+    forall data, predicate data -> decode (encode data) = data.
 
-Definition encode_decode_correct_app
-           (data_t : Type)
-           (encode : data_t -> bin)
-           (decode : bin -> data_t * bin) :=
-  forall data ext, decode (encode data ++ ext) = (data, ext).
+  Class decoder
+        (predicate : data_t -> Prop)
+        (encode : data_t -> bin_t) :=
+  { decode : bin_t -> data_t;
+    decode_correct : encode_decode_correct predicate encode decode }.
 
-Infix "<++>" := encode_decode_correct_app (at level 20, no associativity).
+End Specifications.
 
-Definition encode_decode_correct_app_curry
-           (data_t prev_t proj_t : Type)
-           (prev : data_t -> prev_t)
-           (proj : data_t -> proj_t)
-           (encode : proj_t -> bin)
-           (decode : prev_t -> bin -> proj_t * bin) :=
-  forall data ext, decode (prev data) (encode (proj data) ++ ext) = (proj data, ext).
-
-(* Notation "[ data | encode proj <+++> decode prev ]"
-  := (encode_decode_correct_app_curry (fun data => prev) (fun data => proj) encode decode)
-       (at level 20, no associativity). *)
-
-Definition decode_well_founded (A : Type) (decode : bin -> A * bin) :=
-  forall bin, length (snd (decode bin)) <= pred (length bin).
-
-Class decoder
-      (A : Type)
-      (encode : A -> bin) :=
-  { decode : bin -> A;
-    decode_correct : encode <+> decode }.
-
-Class decoder_block
-      (A : Type)
-      (encode : A -> bin) :=
-  { decode_block : bin -> A * bin;
-    decode_block_app : encode <++> decode_block;
-    decode_block_wellfounded  : decode_well_founded decode_block }.
+Infix "<+>" := (encode_decode_correct (fun _ => True)) (at level 20, no associativity).
