src/BinEncoders/Examples/Sample2.v
@@ -1,0 +1,82 @@
+Require Import Fiat.BinEncoders.Specs
+               Fiat.BinEncoders.Libraries.Core
+               Fiat.BinEncoders.Libraries.FixInt.
+
+Set Implicit Arguments.
+
+Section Sample2.
+
+  Variable List_encode : forall (A : Type) (encode_A : A -> bin), list A -> bin.
+  Variable Nat_encode : nat -> bin.
+
+  Global Instance List_decoder
+         (A : Type)
+         (encode_A : A -> bin)
+         (A_Decoder : decoder (fun _ => True) encode_A)
+         (size : nat)
+    : decoder (fun data => length data = size) (List_encode encode_A).
+  Admitted.
+
+  Global Instance Nat_decoder
+    : decoder (fun _ => True) Nat_encode.
+  Admitted.
+
+  Global Instance App_decoder2
+         (A : Type)
+         (encode_A : A -> bin)
+         (A_Decoder : decoder (fun _ => True) encode_A)
+    : decoder (fun _ => True)
+              (fun _bundle : A * bin => let (_data, _bin) := _bundle in encode_A _data ++ _bin).
+  Admitted.
+
+  Global Instance App_decoder'
+         (A : Type)
+         (encode_A : A -> bin)
+         (predicate : A -> Prop)
+         (A_Decoder : decoder predicate encode_A)
+    : decoder (fun data => predicate (fst data))
+              (fun _bundle : A * bin => let (_data, _) := _bundle in encode_A _data).
+  Admitted.
+
+  Definition DepSS_encode (data : list nat) :=
+    Nat_encode (length data) ++ (List_encode Nat_encode data).
+
+  Definition DepSS_decode :
+    { DepSS_decode | DepSS_encode <+> DepSS_decode }.
+  Proof.
+    unfold DepSS_encode.
+    eexists.
+
+    match goal with
+    | |- encode_decode_correct _ (fun data => ?e1 (_ data) ++ @?e2 data) _ =>
+        eapply decode_unpack with
+           (encode1:=fun (_bundle : _ * bin) =>
+                       let (_proj, _bin) := _bundle
+                       in  e1 _proj ++ _bin)
+           (encode2:=e2)
+    end.
+    instantiate (1:=fun _ => True). intuition. cbv beta. eapply decode_correct. intro len.
+
+
+    match goal with
+    | |- encode_decode_correct _ (fun data => ?e1 data) _ =>
+        eapply decode_unpack with
+           (encode1:=fun (_bundle : _ * bin) =>
+                       let (_proj, _) := _bundle
+                       in  e1 _proj)
+           (encode2:=fun _ => nil)
+    end.
+    instantiate (1:=fun data => length data = len).
+    intuition. cbv beta.
+    (* eapply decode_correct without the following line does not solve it. *)
+    change (fun data : list nat * bin => length (fst data) = len) with
+            (fun data : list nat * bin => (fun ls => length ls = len) (fst data)).
+    eapply decode_correct. intro ls.
+
+    unfold encode_decode_correct.
+    intros.
+    instantiate (1:=fun _ _ => _).
+    simpl in *. intuition. subst. reflexivity.
+  Defined.
+
+End Sample2.
