src/BinEncoders/Libraries/Core.v
@@ -1,0 +1,41 @@
+Require Import Fiat.BinEncoders.Specs.
+
+Definition bin := list bool.
+
+Section Lemmas.
+
+  Lemma decode_unpack
+         (data_t : Type)
+         (bin_t  : Type)
+         (proj_t : Type) :
+    forall (project : data_t -> proj_t)
+           (predicate  : data_t -> Prop)
+           (predicate' : proj_t -> Prop)
+           (encode1 : proj_t * bin_t -> bin_t)
+           (encode2 : data_t -> bin_t)
+           (decode1 : bin_t -> proj_t * bin_t)
+           (decode2 : proj_t -> bin_t -> data_t),
+      (forall data, predicate data -> predicate' (project data)) ->
+      (encode_decode_correct
+         (fun data => predicate' (fst data)) encode1 decode1) ->
+      (forall proj,
+          encode_decode_correct
+            (fun data => predicate data /\ project data = proj) encode2 (decode2 proj)) ->
+      (encode_decode_correct
+         predicate
+         (fun data => encode1 (project data, encode2 data))
+         (fun bin  => let (_proj, _bin) := decode1 bin
+                      in  decode2 _proj _bin)).
+  Proof.
+    unfold encode_decode_correct.
+    intros project predicate predicate' encode1 encode2 decode1 decode2
+           predicate_pf decode1_pf decode2_pf data pred.
+    destruct (decode1 (encode1 (project data, encode2 data))) as [_proj _bin] eqn: eq.
+    specialize (decode1_pf (project data, encode2 data)).
+    specialize (decode2_pf _proj data).
+    rewrite decode1_pf in eq; [ | eapply predicate_pf; eauto ].
+    rewrite <- decode2_pf.
+    inversion eq. eauto. inversion eq. eauto.
+  Qed.
+
+End Lemmas.
